make better use of the succ constructor

our_cook/cbpv.v
@@ -17,15 +17,13 @@ with value : Type :=
 
 Definition id (n : nat) := n.
 
-Definition shift (n : nat) := n + 1.
-
 Definition extend_rn (s : nat) (rn : nat -> nat) (n : nat) := 
   match n with
   | 0 => s
   | S n => rn n
   end.
 
-Definition lift_rn (rn : nat -> nat) := extend_rn 0 (rn >>> shift).
+Definition lift_rn (rn : nat -> nat) := extend_rn 0 (rn >>> S).
 
 Fixpoint int_rn (s : term) (rn : nat -> nat) :=
   match s with
@@ -61,7 +59,7 @@ Definition compose_subst_int_rn
   := int_rn_value (subst n) rn.
 
 Definition lift_subst (subst : nat -> value) := 
-  extend_subst_lam (Var 0) (compose_subst_int_rn subst shift).
+  extend_subst_lam (Var 0) (compose_subst_int_rn subst S).
 
 Notation "^ subst" := (lift_subst subst) (at level 81, left associativity).
 
